extraction/extraction.v
@@ -37,6 +37,8 @@ Require Parser.
 Require Initializers.
 (* Backtranslation *)
 Require Backtranslation.
+(* Capability backend *)
+Require CapAsmgen.
 
 (* Standard lib *)
 Require Import ExtrOcamlBasic.
@@ -125,6 +127,7 @@ Extract Constant Compiler.print_RTL => "PrintRTL.print_if".
 Extract Constant Compiler.print_LTL => "PrintLTL.print_if".
 Extract Constant Compiler.print_Mach => "PrintMach.print_if".
 (* Extract Constant Compiler.print_Asm => "PrintAsm.print_if". *)
+Extract Constant Compiler.print_CapAsm => "PrintCapAsm.print_if".
 Extract Constant Compiler.print => "fun (f: 'a -> unit) (x: 'a) -> f x; x".
 Extract Constant Compiler.time  => "Timing.time_coq".
 
@@ -143,6 +146,7 @@ Extract Constant Cabs.char_code => "int64".
 (* Processor-specific extraction directives *)
 
 Load extractionMachdep.
+Load CapextractionMachdep.
 
 (* Avoid name clashes *)
 Extraction Blacklist List String Int.
@@ -156,6 +160,7 @@ Cd "extraction".
 
 Separate Extraction
    Compiler.transf_c_program Compiler.transf_cminor_program
+   CapAsmgen.transf_program
    Cexec.do_initial_state Cexec.do_step Cexec.at_final_state
    Ctypes.merge_attributes Ctypes.remove_attributes 
    Ctypes.build_composite_env Ctypes.layout_struct
